Lean4Axiomatic/Natural/Impl/Generic/Core.lean
@@ -1,0 +1,31 @@
+import Lean4Axiomatic.Natural.Core
+
+/-! # Generic implementation of core natural number properties -/
+
+namespace Lean4Axiomatic.Natural.Impl.Generic
+
+variable {ℕ : Type} [Constructor.Ops ℕ] [Equality ℕ]
+
+/--
+Convert a `Nat` value to its equivalent `ℕ` value.
+
+Lean's prelude defines `Nat` as its natural number type, so it's useful to have
+a way to translate from it. In particular, numeric literals are represented
+as `Nat` values, so if we want to have literals for `ℕ`, we need to convert.
+See the `OfNat` instance below for more details.
+-/
+def fromNat : Nat → ℕ
+| 0 => zero
+| n+1 => step (fromNat n)
+
+def ofNat {n : Nat} : OfNat ℕ n := {
+  ofNat := fromNat n
+}
+
+def literals : Literals ℕ := {
+  literal := ofNat
+  literal_zero := Rel.refl
+  literal_step := Rel.refl
+}
+
+end Lean4Axiomatic.Natural.Impl.Generic
