Lean4Axiomatic/Natural/Impl/Generic/Exponentiation.lean
@@ -1,0 +1,60 @@
+import Lean4Axiomatic.Natural.Exponentiation
+
+/-!
+# Generic implementation of natural number exponentiation and properties
+-/
+
+namespace Lean4Axiomatic.Natural.Impl.Generic
+
+open Relation.Equivalence (EqvOp)
+
+variable
+  {ℕ : Type} [Core ℕ] [Induction.{1} ℕ] [Addition ℕ] [Multiplication ℕ]
+  {α : Type} [EqvOp α] [OfNat α 1] [Mul α]
+
+/--
+Raise a value to a natural number power.
+
+**Definition intuition**: Performs the correct number of multiplications using
+recursion.
+-/
+def _pow (x : α) (n : ℕ) : α := rec_on n 1 (· * x)
+
+local instance exponentiation_ops : Exponentiation.Ops α ℕ := {
+  _pow := _pow
+}
+
+/--
+Anything to the zero power is one.
+
+**Property and proof intuition**: This corresponds to the base case in the
+recursive definition of `_pow`.
+-/
+theorem pow_zero {x : α} : x ^ (0:ℕ) ≃ 1 := calc
+  _ ≃ x ^ (0:ℕ)          := Rel.refl
+  _ = rec_on 0 1 (· * x) := rfl
+  _ = 1                  := rec_on_zero
+
+/--
+Adding one to the exponent multiplies the result by the base.
+
+**Property and proof intuition**: This corresponds to the recursive case in the
+definition of `_pow`.
+-/
+theorem pow_step {x : α} {n : ℕ} : x ^ step n ≃ x ^ n * x := calc
+  _ ≃ x ^ step n                := Rel.refl
+  _ = rec_on (step n) 1 (· * x) := rfl
+  _ = (rec_on n 1 (· * x)) * x  := rec_on_step
+  _ = x ^ n * x                 := rfl
+
+def exponentiation_props : Exponentiation.Props (α := α) (· * ·) := {
+  pow_zero := pow_zero
+  pow_step := pow_step
+}
+
+def exponentiation : Exponentiation ℕ (α := α) (· * ·) := {
+  toOps := exponentiation_ops
+  toProps := exponentiation_props
+}
+
+end Lean4Axiomatic.Natural.Impl.Generic
