Lean4Axiomatic/Natural/Impl/Generic/Order.lean
@@ -1,0 +1,15 @@
+import Lean4Axiomatic.Natural.Addition
+
+/-! # Generic implementation of natural number order relations -/
+
+namespace Lean4Axiomatic.Natural.Impl.Generic
+
+variable {ℕ : Type} [Core ℕ] [Addition ℕ]
+
+def le (n m : ℕ) : Prop := ∃ k : ℕ, n + k ≃ m
+local instance le_ex_add : LE ℕ := LE.mk le
+
+def lt (n m : ℕ) : Prop := n ≤ m ∧ n ≄ m
+def lt_le_neqv : LT ℕ := LT.mk lt
+
+end Lean4Axiomatic.Natural.Impl.Generic
