Lean4Axiomatic/Natural/Impl/Generic/Sign.lean
@@ -1,0 +1,22 @@
+import Lean4Axiomatic.Natural.Sign
+import Lean4Axiomatic.Sign
+
+/-! # Generic implementation of natural number signedness properties -/
+
+namespace Lean4Axiomatic.Natural.Impl.Generic
+
+variable {ℕ : Type} [Core ℕ]
+
+def positive_ops : Signed.Positivity.Ops ℕ := {
+  Positive := λ n => n ≄ 0
+}
+
+def positivity : Signed.Positivity ℕ := {
+  positive_defn := Iff.intro id id
+}
+
+def sign : Sign ℕ := {
+  positivity := positivity
+}
+
+end Lean4Axiomatic.Natural.Impl.Generic
