Lean4Axiomatic/Rational/Impl/Fraction.lean
@@ -1,3 +1,4 @@
+import Lean4Axiomatic.Natural.Impl.Generic
 import Lean4Axiomatic.Rational
 import Lean4Axiomatic.Rational.Impl.Fraction.Reciprocation
 import Lean4Axiomatic.Rational.Impl.Fraction.Sign
@@ -9,8 +10,8 @@ import Lean4Axiomatic.Rational.Impl.Generic.Order
 
 namespace Lean4Axiomatic.Rational.Impl.Fraction
 
-variable {ℕ : Type} [Natural ℕ]
-variable {ℤ : Type} [Integer (ℕ := ℕ) ℤ]
+variable
+  {ℕ ℤ : Type} [Natural ℕ] [Natural.Induction.{1} ℕ] [Integer (ℕ := ℕ) ℤ]
 
 instance rational : Rational (ℤ := ℤ) (Fraction ℤ) :=
   let order := Generic.order
@@ -19,6 +20,7 @@ instance rational : Rational (ℤ := ℤ) (Fraction ℤ) :=
     toCore := core
     toAddition := addition
     toMultiplication := multiplication
+    toExponentiation := Natural.Impl.Generic.exponentiation
     toNegation := negation
     toSubtraction := subtraction
     toReciprocation := reciprocation
